```{r setup}
#| message: false
#| warning: false
```

## Differential equation {.unnumbered}

We want to solve the following differential equation $E$:

$$y'(t) = STP(t) - \alpha\cdot exp(-\lambda \cdot t) + (\omega_P-\omega_M) \cdot y(t)$$

with: 

$$STP(t) = \delta\left(\frac{t}{\tau}\cdot exp(1-\frac{t}{\tau})\right)^2$$

The general solution of differential equation $E_0$:

$$y'(t) - (\omega_P-\omega_M) \cdot y(t) = 0$$

is $y_G = Kexp((\omega_P-\omega_M) t)$

A particular solution of differential equation $E_1$:

$$y'(t) - (\omega_P-\omega_M) \cdot y(t) = \alpha\cdot exp(-\lambda\cdot t)$$

is

$$y_{p1} = -\frac{\alpha}{(\omega_P-\omega_M)+\lambda} \cdot exp(-\lambda\cdot t)$$

A particular solution of differential equation $E_2$:

$$y'(t) - (\omega_P-\omega_M) \cdot y(t) = \delta \left(\frac{t}{\tau}exp(1-\frac{t}{\tau})\right)^2$$

is

$$y_{p2} = exp(1-\frac{t}{\tau})^2\frac{2\delta}{\tau^2(-2(\omega_P-\omega_M)-\tau)}\left(t^2 - t\frac{4}{(-2(\omega_P-\omega_M)-\tau)} + \frac{8}{(-2(\omega_P-\omega_M)-\tau)^2}\right)$$

The general solution to differential equation (E) is therefore:

$$y(t) = Kexp(-(\omega_P-\omega_M) t) -\frac{\alpha}{(\omega_P-\omega_M)+\lambda} \cdot exp(-\lambda\cdot t) + exp(1-\frac{t}{\tau})^2\frac{2\delta}{\tau^2(-2(\omega_P-\omega_M)-\tau)}\left(t^2 - t\frac{4}{(-2(\omega_P-\omega_M)-\tau)} + \frac{8}{(-2(\omega_P-\omega_M)-\tau)^2}\right)$$

$$ K = y_0+ \frac{\alpha}{(\omega_P-\omega_M)+\lambda} -\frac{16e^2\delta}{\tau^2(2(\omega_P-\omega_M)-\tau)^3}$$
